src/crypto/poly1305/x64/X64.Poly1305.Math_i.fsti
@@ -37,17 +37,17 @@ let memModified (old_mem:mem) (new_mem:mem) (ptr:int) (num_bytes) =
     
 let heapletTo128 (m:mem) (i:int) (len:nat) : (int->nat128) =
   fun addr -> if i <= addr && addr < (i + len) && (addr - i) % 16 = 0 then m.[addr] + 0x10000000000000000 * m.[addr + 8] else 42
-
+(*
 val heapletTo128_preserved (m:mem) (m':mem) (i:int) (len:nat) : Lemma 
-  (requires  (forall (a:int) . m `Map.contains` a <==> m' `Map.contains` a) /\
-             (forall (a:int) .  m' `Map.contains` a /\ (i <= a) /\ a < (i + len) ==> m.[a] == m'.[a]))
+  (requires memModified m m' ptr num_bytes /\
+            disjoint ptr num_bytes i ((len + 15) / 16 * 16))
   (ensures  heapletTo128 m i len == heapletTo128 m' i len)
-             
-val heapletTo128_all_preserved (m:mem) (i:int) (len:nat) : Lemma 
+ *)            
+val heapletTo128_all_preserved (m:mem) (ptr num_bytes i:int) (len:nat) : Lemma 
   (requires True)
   (ensures (forall (m':mem) .
-             (forall (a:int) . m `Map.contains` a <==> m' `Map.contains` a) /\
-             (forall (a:int) .  m' `Map.contains` a /\ (i <= a) /\ a < (i + len) ==> m.[a] == m'.[a])
+              memModified m m' ptr num_bytes /\
+              disjoint ptr num_bytes i ((len + 15) / 16 * 16)
              ==>
              heapletTo128 m i len == heapletTo128 m' i len))
 
